wip

Foundation/Modal/Kripke/Hilbert/GrzPoint2.lean
@@ -1,5 +1,6 @@
 import Foundation.Modal.Kripke.Hilbert.Grz.Completeness
 import Foundation.Modal.Kripke.Hilbert.S4Point2
+import Mathlib.Data.Finite.Sum
 
 namespace LO.Modal
 
@@ -9,6 +10,82 @@ open Formula
 open Formula.Kripke
 open Hilbert.Kripke
 open Kripke
+
+namespace Formula
+
+variable {α} [DecidableEq α]
+variable {φ : Formula α} {a : α}
+
+def atoms : Formula α → Finset α
+  | ⊥ => ∅
+  | .atom v => {v}
+  | □φ => φ.atoms
+  | φ ➝ ψ => φ.atoms ∪ ψ.atoms
+
+lemma iff_mem_atoms_mem_subformula : (a ∈ φ.atoms) ↔ (atom a ∈ φ.subformulas) := by
+  induction φ using Formula.rec' <;> simp_all [atoms, subformulas];
+
+end Formula
+
+
+section
+
+namespace Kripke
+
+def Frame.terminals (F : Frame) : Set F.World := { t | ∀ {y}, t ≺ y → y = t }
+def Frame.terminals_of (F : Frame) (x : F.World) : Set F.World := { t | x ≺^+ t ∧ ∀ {y}, t ≺ y → y = t }
+
+end Kripke
+
+namespace Formula.Kripke.Satisfies
+
+variable {F V} {φ : Formula ℕ}
+
+lemma box_at_terminal {x : F.World} (hx : x ∈ F.terminals) (h : Satisfies ⟨F, V⟩ x φ) : Satisfies ⟨F, V⟩ x (□φ) := by
+  intro y Rxy;
+  have := hx Rxy;
+  subst this;
+  exact h;
+
+lemma dia_at_terminal {x : F.World} (hx : x ∈ F.terminals) (h :  ¬Satisfies ⟨F, V⟩ x φ) : ¬Satisfies ⟨F, V⟩ x (◇φ) := by
+  simp [Satisfies, Frame.terminals, not_exists, Set.mem_setOf_eq, Satisfies] at hx ⊢;
+  intro y Rxy;
+  have := hx Rxy;
+  subst this;
+  exact h;
+
+end Formula.Kripke.Satisfies
+
+end
+
+
+section
+
+namespace Hilbert
+
+open Entailment
+
+lemma Grz_weakerThan_GrzPoint2 : Hilbert.Grz ⪯ Hilbert.GrzPoint2 := weakerThan_of_dominate_axioms $ by simp;
+
+lemma GrzPoint2_of_Grz (h : (φ.atoms.image (λ a => Axioms.Point2 (.atom a))).toSet *⊢[Hilbert.Grz]! φ) : Hilbert.GrzPoint2 ⊢! φ := by
+  obtain ⟨Γ, hΓ₁, hΓ₂⟩ := Context.provable_iff.mp h;
+  simp at hΓ₁;
+  replace hΓ₂ := Grz_weakerThan_GrzPoint2.pbl $ FiniteContext.provable_iff.mp hΓ₂;
+  exact hΓ₂ ⨀ by
+    apply conj_intro'!;
+    intro γ hγ;
+    obtain ⟨a, ha, rfl⟩ := hΓ₁ _ hγ;
+    exact axiomPoint2!;
+
+lemma not_Grz_of_not_GrzPoint2 (h : Hilbert.GrzPoint2 ⊬ φ) : (φ.atoms.image (λ a => Axioms.Point2 (.atom a))).toList ⊬[Hilbert.Grz] φ := by
+  have := provable_iff.not.mp $ not_imp_not.mpr GrzPoint2_of_Grz h;
+  push_neg at this;
+  convert this ((φ.atoms.image (λ a => Axioms.Point2 (.atom a))).toList) $ by simp;
+
+end Hilbert
+
+end
+
 
 namespace Kripke
 
@@ -44,41 +121,174 @@ instance finite_sound : Sound (Hilbert.GrzPoint2) FrameClass.finite_confluent_pa
 instance consistent : Entailment.Consistent (Hilbert.GrzPoint2) :=
   consistent_of_sound_frameclass FrameClass.finite_confluent_partial_order (by simp)
 
-instance finite_complete : Complete (Hilbert.GrzPoint2) FrameClass.finite_confluent_partial_order :=
-  Kripke.Grz.complete_of_mem_miniCanonicalFrame FrameClass.finite_confluent_partial_order $ by
-    sorry
-    /-
-    intro φ;
-    refine ⟨miniCanonicalFrame.reflexive, miniCanonicalFrame.transitive, miniCanonicalFrame.antisymm, ?_⟩;
-    intro X Y Z ⟨⟨RXY₁, RXY₂⟩, ⟨RXZ₁, RXZ₂⟩⟩;
-    obtain ⟨U, hU⟩ := ComplementClosedConsistentFinset.lindenbaum (𝓢 := Hilbert.GrzPoint2) (Φ := Y.1 ∪ Z.1) (Ψ := φ.subformulasGrz)
-      (by
-        apply Finset.union_subset_iff.mpr;
+
+section
+
+open Relation
+
+instance finite_complete : Complete (Hilbert.GrzPoint2) FrameClass.finite_confluent_partial_order := ⟨by
+  intro φ;
+  contrapose;
+  intro hφ;
+
+  replace hφ : Hilbert.Grz ⊬ ⋀((φ.atoms.image (λ a => Axioms.Point2 (atom a))).toList) ➝ φ := not_Grz_of_not_GrzPoint2 hφ;
+  generalize eΓ : (φ.atoms.image (λ a => Axioms.Point2 (atom a))).toList = Γ at hφ;
+  obtain ⟨M, r, ⟨_, M_refl, M_trans, M_antisymm⟩, hΓφ⟩ := exists_model_world_of_not_validOnFrameClass $ not_imp_not.mpr (@Hilbert.Grz.Kripke.complete.complete _) hφ;
+
+  clear hφ;
+
+  let RM := M↾r;
+  let r' : RM.World := ⟨r, by tauto⟩;
+  have RM_rooted : ∀ (w : RM.World), r' ≺ w := by
+    intro w;
+    by_cases e : r' = w;
+    . subst e; apply Frame.pointGenerate.rel_refl M_refl;
+    . exact TransGen.unwrap (Frame.pointGenerate.rel_trans M_trans) (Frame.IsRooted.root_generates w (by tauto));
+
+  replace hΓφ : ¬(r' ⊧ ⋀Γ → r' ⊧ φ) := Satisfies.imp_def.not.mp $ Model.pointGenerate.modal_equivalent_at_root (r := r) |>.not.mpr hΓφ;
+  push_neg at hΓφ;
+  obtain ⟨hΓ, hφ⟩ := hΓφ;
+
+  let M' : Kripke.Model := {
+    World := RM.World ⊕ Unit
+    Rel x y :=
+      match x, y with
+      | _, (Sum.inr _) => True
+      | (Sum.inl x), (Sum.inl y) => RM.Rel x y
+      | _, _ => False
+    Val x a :=
+      match x with
+      | Sum.inl x => RM.Val x a
+      | _ => ∀ y ∈ RM.toFrame.terminals, RM.Val y a
+  };
+  apply not_validOnFrameClass_of_exists_model_world;
+  use M', (Sum.inl r');
+  constructor;
+  . refine ⟨?_, ?_, ?_, ?_, ?_⟩;
+    . apply Frame.isFinite_iff _ |>.mpr;
+      infer_instance;
+    . intro x;
+      match x with
+      | Sum.inl x => apply M_refl;
+      | Sum.inr x => simp_all [M'];
+    . intro x y z Rxy Ryz;
+      match x, y, z with
+      | Sum.inl x, Sum.inl y, Sum.inl z => exact Frame.pointGenerate.rel_trans M_trans Rxy Ryz;
+      | _, _, Sum.inr z => simp_all [M'];
+      | _, Sum.inr y, Sum.inl z => simp_all [M'];
+    . intro x y Rxy Ryz;
+      match x, y with
+      | Sum.inl x, Sum.inl y =>
+        simp only [Sum.inl.injEq, M'];
+        exact Frame.pointGenerate.rel_antisymm M_antisymm Rxy Ryz;
+      | Sum.inl x, Sum.inr y => simp_all [M'];
+      | Sum.inr x, Sum.inr y => simp_all [M'];
+      | Sum.inr x, Sum.inl y => simp_all [M'];
+    . rintro x y z ⟨Rxy, Ryz⟩;
+      use (Sum.inr ());
+      simp [M'];
+  . have H₁ : ∀ a ∈ φ.atoms, ∀ t ∈ RM.toFrame.terminals, ∀ t' ∈ RM.toFrame.terminals, RM t a → RM t' a := by
+      intro a ha t t_terminal t' t'_terminal hy;
+      by_contra hy';
+      have : ¬t' ⊧ (◇atom a) := Kripke.Satisfies.dia_at_terminal t'_terminal hy';
+      have : ¬r' ⊧ □(◇atom a) := by
+        apply Satisfies.box_def.not.mpr;
+        push_neg;
+        use t';
         constructor;
-        . intro ψ hψ; exact Y.2.2 |>.subset hψ;
-        . intro ψ hψ; exact Z.2.2 |>.subset hψ;
-      )
-      (by
-        simp [FormulaFinset.Consistent];
-        sorry;
-      );
-    use U;
-    constructor;
-    . constructor;
-      . intro ψ _ hψY; exact hU $ Finset.mem_union.mpr (by tauto);
-      . intro h;
-        ext ξ;
+        . apply RM_rooted;
+        . assumption;
+      have : ¬r' ⊧ ◇(□atom a) := by
+        revert this;
+        apply not_imp_not.mpr
+        exact Satisfies.conj_def.mp hΓ (Axioms.Point2 (atom a)) (by simpa [←eΓ]);
+      have := Satisfies.dia_def.not.mp this;
+      push_neg at this;
+      have : ¬t ⊧ □atom a := this t (RM_rooted t);
+      have : t ⊧ □atom a := Kripke.Satisfies.box_at_terminal t_terminal hy;
+      contradiction;
+    have H₂ : ∀ t ∈ RM.terminals, ∀ ψ ∈ φ.subformulas, t ⊧ ψ ↔ (Satisfies M' (Sum.inr ()) ψ) := by
+      intro t t_terminal ψ ψ_sub;
+      induction ψ using Formula.rec' with
+      | hatom a =>
+        simp [Satisfies, M']
         constructor;
-        . intro hξY; exact hU $ Finset.mem_union.mpr (by tauto);
-        . sorry;
-    . constructor;
-      . intro ψ _ hψZ; exact hU $ Finset.mem_union.mpr (by tauto);
-      . intro h;
-        ext ξ;
+        . intro ha t' t'_terminal;
+          exact H₁ a (iff_mem_atoms_mem_subformula.mpr ψ_sub) t t_terminal t' t'_terminal ha;
+        . intro h;
+          apply h;
+          exact t_terminal;
+      | hfalsum => tauto;
+      | himp χ ξ ihχ ihξ =>
         constructor;
-        . intro hξZ; exact hU $ Finset.mem_union.mpr (by tauto);
-        . sorry;
-    -/
+        . intro h hχ;
+          apply ihξ (Formula.subformulas.mem_imp₂ ψ_sub) |>.mp;
+          apply h;
+          apply ihχ (Formula.subformulas.mem_imp₁ ψ_sub) |>.mpr;
+          assumption;
+        . intro h hχ;
+          apply ihξ (Formula.subformulas.mem_imp₂ ψ_sub) |>.mpr;
+          apply h;
+          apply ihχ (Formula.subformulas.mem_imp₁ ψ_sub) |>.mp;
+          assumption;
+      | hbox ψ ihψ =>
+        constructor;
+        . intro ht u Ru;
+          match u with
+          | Sum.inl x => simp [M', Frame.Rel'] at Ru;
+          | Sum.inr _ =>
+            apply ihψ (Formula.subformulas.mem_box ψ_sub) |>.mp;
+            apply ht;
+            apply Frame.pointGenerate.rel_refl M_refl;
+        . intro ht u Rtu;
+          have := t_terminal Rtu; subst this;
+          apply ihψ (Formula.subformulas.mem_box ψ_sub) |>.mpr;
+          apply ht;
+          tauto;
+    have : ∀ y : RM.World, ∀ ψ ∈ φ.subformulas, y ⊧ ψ ↔ (Satisfies M' (Sum.inl y) ψ) := by
+      intro y ψ ψ_sub;
+      induction ψ using Formula.rec' generalizing y with
+      | hbox ψ ihψ =>
+        constructor;
+        . intro hψ v Ruv;
+          match v with
+          | Sum.inl x =>
+            simp [M', Frame.Rel'] at Ruv;
+            exact ihψ x (Formula.subformulas.mem_box ψ_sub) |>.mp $ hψ _ Ruv;
+          | Sum.inr x =>
+            obtain ⟨t, t_terminal, Rut⟩ : ∃ t ∈ RM.terminals, y ≺ t := by sorry
+              /-
+              by_contra hC;
+              push_neg at hC;
+              simp [Frame.terminals] at hC;
+              by_cases y_terminal : y ∈ RM.terminals;
+              . exact hC y y_terminal $ Frame.pointGenerate.rel_refl M_refl y;
+              . simp [Frame.terminals] at y_terminal;
+                obtain ⟨z, Ryz, eyz⟩ := y_terminal;
+                by_cases z_terminal : z ∈ RM.terminals;
+                . exact hC z z_terminal Ryz;
+                . simp [Frame.terminals] at z_terminal;
+                  obtain ⟨w, Rzw, ewz⟩ := z_terminal;
+                  have ewy : w ≠ y := by
+                    by_contra ewy; subst ewy;
+                    have := Frame.pointGenerate.rel_antisymm M_antisymm Rzw Ryz;
+                    contradiction;
+                  -- by similar arguments, arbitary n-poinst in RM, but FM is finite. it contradicts.
+              -/
+            apply H₂ t t_terminal ψ (Formula.subformulas.mem_box ψ_sub) |>.mp;
+            apply hψ;
+            exact Rut;
+        . intro h v Ruv;
+          exact ihψ v (Formula.subformulas.mem_box ψ_sub) |>.mpr $ @h (Sum.inl v) Ruv;
+      | himp _ _ ihχ ihξ =>
+        have := ihχ y (Formula.subformulas.mem_imp₁ ψ_sub);
+        have := ihξ y (Formula.subformulas.mem_imp₂ ψ_sub);
+        tauto;
+      | _ => tauto;
+    exact this r' φ (by simp) |>.not.mp hφ;
+⟩
+
+end
 
 end Hilbert.GrzPoint2.Kripke
 
